Verify concrete chat server; admits remain

adequacy.v
@@ -13,14 +13,28 @@ Class heapIPreG Σ := HeapIPreG {
   ioI_exclG :> inG Σ io_monoid;
 }.
 
+Class heapIPreIOG Σ := HeapIPreIOG {
+  heapI_invPreIOG :> invG Σ;
+  heapI_gen_heapPreIOG :> gen_heapG loc val Σ;
+  prophI_gen_heapPreIOG :> gen_heapG loc (Stream val) Σ;
+  ioI_exclPreIOG :> inG Σ io_monoid;
+}.
+
+Definition make_heapIG `{heapIPreIOG Σ} γio : heapIG Σ := {| γio := γio |}.
+
 Definition IoΣ := #[invΣ; gen_heapΣ loc val; gen_heapΣ loc (Stream val);
                       GFunctor io_monoid].
 
 Global Instance subG_io_monoid Σ : subG IoΣ Σ → inG Σ io_monoid.
 Proof. solve_inG. Qed.
 
+Global Instance subG_heapIPreG Σ : subG IoΣ Σ → heapIPreG Σ.
+Proof. solve_inG. Qed.
+
 Theorem adequacy_instrumented Σ `{heapIPreG Σ} e Φ M :
-  (∀ `{Hig : heapIG Σ}, (WP e @ NotStuck; ⊤ {{ Φ }})%I) → safe e M.
+  (∀ `{Hig : heapIPreIOG Σ},
+      (|={⊤}=> ∃ γio, let _ := make_heapIG γio in
+             FullIO M ∗ WP e @ NotStuck; ⊤ {{ Φ }})%I) → safe e M.
 Proof.
   intros Hwp.
   cut (adequate NotStuck e {| Heap := ∅; Proph := ∅; ioState := M |} (λ _, True)).
@@ -29,21 +43,24 @@ Proof.
     specialize (Hns th2 σ2 e' eq_refl Hrtc He'); eauto. }
   eapply wp_adequacy; first apply _.
   iIntros (Hinv) "".
-  iMod (@own_alloc _ io_monoid _ (● Excl' (M : leibnizC ioSpec)))
-    as (γio) "HGI".
-  { split; last done. intros n; eapply ucmra_unit_leastN. }
   iMod (gen_heap_init (∅ : gmap loc val)) as (Hheap) "Hheap".
   iMod (gen_heap_init (∅ : gmap loc (Stream val))) as (Hproph) "Hproph".
-  set (HIG := {| γio := γio |} : heapIG Σ).
+  pose ({| heapI_invPreIOG := _ |}).
+  iMod (Hwp _) as (γio) "[HFIO Hwp]".
+  pose ({| γio := γio |}).
   iModIntro.
   iExists heapIG_stateI.
-  iSplitL; first by iFrame.
-    by (iApply wp_mono; last iApply Hwp; eauto).
+  iSplitR "Hwp"; first by iFrame.
+  iApply (wp_mono); last by iApply "Hwp".
+  eauto.
 Qed.
 
 Theorem adequacy Σ `{heapIPreG Σ} (e : expr) Φ M :
   prefix_closed M →
-  (∀ `{Hig : heapIG Σ}, (WP e @ NotStuck; ⊤ {{ Φ }})%I) → fully_erased_safe e M.
+  (∀ `{Hig : heapIPreIOG Σ},
+      (|={⊤}=> ∃ γio, let _ := make_heapIG γio in
+                     FullIO M ∗ WP e @ NotStuck; ⊤ {{ Φ }})%I) →
+  fully_erased_safe e M.
 Proof.
   intros HPC Hig.
   apply soundness_io; eauto.
