chat_server_concrete.v
@@ -1,0 +1,422 @@
+From iris.algebra Require Import auth.
+From iris.proofmode Require Import tactics.
+From iris.base_logic Require Import fixpoint.
+From iris.program_logic Require Import weakestpre lifting.
+From iris_io Require Import lang rules abstract_petrinet petrinet
+     chat_server channel adequacy.
+
+Section conrete_chat_server.
+  Context `{heapIG Σ, petrinetIG Σ, channelIG Σ}.
+
+  Definition read_nick1 := 1%positive.
+  Definition read_nick2 := 2%positive.
+
+  Definition write_nick1 := 1%positive.
+  Definition write_nick2 := 2%positive.
+
+  Definition bool_to_write_tag (b : bool) :=
+    if b then write_nick1 else write_nick2.
+
+  Definition to_write_tag :=
+    Lam (If (Var 0) (IOtag write_nick1) (IOtag write_nick2)).
+
+  Lemma wp_to_write_tag b :
+    {{{ True }}}
+      App to_write_tag (Bool b)
+    {{{ RET (IOtagV (bool_to_write_tag b)); True }}}.
+  Proof.
+    iIntros (Φ) "_ HΦ".
+    iApply wp_pure_step_later; trivial.
+    iNext. asimpl.
+    by destruct b;
+      iApply wp_pure_step_later; trivial; iNext;
+        iApply wp_value; iApply "HΦ".
+  Qed.
+
+  Definition bool_to_read_tag (b : bool) :=
+    if b then read_nick1 else read_nick2.
+
+  Definition to_read_tag :=
+    Lam (If (Var 0) (IOtag read_nick1) (IOtag read_nick2)).
+
+  Lemma wp_to_read_tag b :
+    {{{ True }}}
+      App to_read_tag (Bool b)
+    {{{ RET (IOtagV (bool_to_read_tag b)); True }}}.
+  Proof.
+    iIntros (Φ) "_ HΦ".
+    iApply wp_pure_step_later; trivial.
+    iNext. asimpl.
+    by destruct b;
+      iApply wp_pure_step_later; trivial; iNext;
+        iApply wp_value; iApply "HΦ".
+  Qed.
+
+  Definition send_to_nick :=
+    Lam (Lam (Seq (IO (App to_write_tag (Var 1)) (Var 0)) Unit)).
+
+  Lemma send_to_nick_closed : ∀ f, send_to_nick.[f] = send_to_nick.
+  Proof. done. Qed.
+
+  Definition receive_from_nick :=
+    Lam ((IO (App to_read_tag (Var 0)) Unit)).
+
+  Lemma receive_from_nick_closed :
+    ∀ f, receive_from_nick.[f] = receive_from_nick.
+  Proof. done. Qed.
+
+  Definition place_stream :=
+    (prodC (leibnizC Places) (leibnizC (Stream val))).
+
+  Definition IO_pre_sequence
+             (io_gen : val → Places → Places -> Transition)
+             (f : place_stream → iProp Σ)
+             (pμ : place_stream) : iProp Σ :=
+    (∃ q, ⌜ThePetriNet (io_gen (Shead (pμ.2)) (pμ.1) q)⌝ ∧
+          f (q, Stail (pμ.2)))%I.
+
+  Global Instance IO_pre_sequence_BIMonoPred io_gen :
+           BIMonoPred (IO_pre_sequence io_gen).
+  Proof.
+    split.
+    - iIntros (Φ Ψ) "#HΦΨ"; iIntros ([p μ]).
+      iDestruct 1 as (q) "[% HPhi]"; simpl in *.
+      iExists q; iSplit; first trivial.
+      by iApply "HΦΨ".
+    - by intros Φ HΦ k [p μ] [p' μ'] [Hp%leibniz_equiv Hμ%leibniz_equiv];
+      simpl in *; subst.
+  Qed.
+
+  Definition IO_sequence io_gen :=
+    uPred_greatest_fixpoint (IO_pre_sequence io_gen).
+
+  Definition ReceiveFromNick :=
+    λ p n μ,
+    match n with
+    | BoolV b =>
+      (IO_sequence (λ v p q, IOTr p (bool_to_read_tag b) UnitV v q) (p, μ))%I
+    | _ => False%I
+    end.
+
+  Definition SendToNick :=
+    λ p n μ,
+    match n with
+    | BoolV b =>
+      (IO_sequence (λ v p q, IOTr p (bool_to_write_tag b) v UnitV q) (p, μ))%I
+    | _ => False%I
+    end.
+
+  Lemma wp_receive_from_nick : ∀ r n m μ,
+    {{{ token r ∗ ReceiveFromNick r n {| Shead := m; Stail := μ|} }}}
+      App receive_from_nick (of_val n)
+    {{{ RET m; ∃ r', token r' ∗ ReceiveFromNick r' n μ }}}.
+  Proof.
+    iIntros (r n m μ Φ) "[Hr Hrfn] HΦ".
+    iApply wp_pure_step_later; trivial.
+    iNext. asimpl.
+    destruct n; simpl; try done.
+    rewrite {1}/IO_sequence greatest_fixpoint_unfold.
+    iDestruct "Hrfn" as (q) "/= [% Hrfn]".
+    iApply (wp_bind (fill [IOLCtx _])).
+    iApply wp_to_read_tag; trivial.
+    iNext; iIntros "_"; simpl.
+    iApply (wp_petrinet_io with "Hr"); eauto.
+    iNext. iIntros "Hq".
+    iApply "HΦ". iExists _; iFrame.
+  Qed.
+
+  Lemma wp_send_to_nick : ∀ s n m μ,
+    {{{ token s ∗ SendToNick s n {| Shead := m; Stail := μ|} }}}
+      App (App send_to_nick (of_val n)) (of_val m)
+    {{{ RET UnitV; ∃ s', token s' ∗ SendToNick s' n μ }}}.
+  Proof.
+    iIntros (r n m μ Φ) "[Hr Hrfn] HΦ".
+    iApply (wp_bind (fill [AppLCtx _])).
+    iApply wp_pure_step_later; trivial.
+    iNext. asimpl. iApply wp_value; simpl.
+    iApply wp_pure_step_later; trivial.
+    iNext. asimpl.
+    destruct n; simpl; try done.
+    rewrite {1}/IO_sequence greatest_fixpoint_unfold.
+    iDestruct "Hrfn" as (q) "/= [% Hrfn]".
+    iApply (wp_bind (fill [SeqCtx _])).
+    iApply (wp_bind (fill [IOLCtx _])).
+    iApply wp_to_read_tag; trivial.
+    iNext; iIntros "_"; simpl.
+    iApply (wp_petrinet_io with "Hr"); eauto.
+    iNext. iIntros "Hq".
+    iApply wp_pure_step_later; trivial.
+    iNext. iApply wp_value.
+    iApply "HΦ". iExists _; iFrame.
+  Qed.
+
+  Global Program Instance concrete_nick_comm_prog : abstract_nick_comm_prog :=
+    {|
+      chat_server.send_to_nick := send_to_nick;
+      chat_server.receive_from_nick := receive_from_nick;
+    |}.
+  Solve Obligations with eauto.
+
+  Global Program Instance concrete_nick_comm : abstract_nick_comm :=
+    {|
+      chat_server.ReceiveFromNick := ReceiveFromNick;
+      chat_server.SendToNick := SendToNick;
+    |}.
+  Solve Obligations with eauto using wp_receive_from_nick, wp_send_to_nick.
+
+  Program Definition concrete_serveChatRoom :=
+    serveChatRoom (BoolV true) (BoolV false).
+
+  Theorem wp_concrete_serverChatRoom r1 r2 s μ1 μ2 :
+    {{{ token r1 ∗ ReceiveFromNick r1 (BoolV true) μ1 ∗
+        token r2 ∗ ReceiveFromNick r2 (BoolV false) μ2 ∗
+        token s ∗ ∀ μ, ⌜interleaving μ1 μ2 μ⌝ →
+                       SendToNicks s (BoolV true) (BoolV false) μ }}}
+      concrete_serveChatRoom
+  {{{RET UnitV; False}}}.
+  Proof.
+    iIntros (Φ) "(Hr1 & Hrf1 & Hr2 & Hrf2 & Hs & Hsnd) HΦ".
+    iApply (wp_serverChatRoom _ _ r1 r2 s with "[-HΦ]"); simpl; eauto.
+    iFrame.
+  Qed.
+
+End conrete_chat_server.
+
+(* Definition make_input_io (tg : ioTag) (μ : Stream val):= *)
+(*   Smap (λ x, (tg, UnitV, x)) μ. *)
+
+(* Definition make_output_io (tg : ioTag) (μ : Stream val):= *)
+(*   Smap (λ x, (tg, x, UnitV)) μ. *)
+
+(* Definition chat_server_io mixer μ1 μ2 μ := *)
+(*   ∃ μwr, *)
+(*     interleaving (make_output_io write_nick1 (Smix mixer μ1 μ2)) *)
+(*                  (make_output_io write_nick2 (Smix mixer μ1 μ2)) μwr ∧ *)
+(*     interleaving (Smix mixer (make_input_io read_nick1 μ1) *)
+(*                        (make_input_io read_nick2 μ2)) μwr μ. *)
+
+(* Definition chat_server_ioSpec mixer μ1 μ2 : ioSpec := *)
+(*   λ l, ∃ μ, chat_server_io mixer μ1 μ2 (append_l_s l μ). *)
+
+Inductive chat_server_petri_places :=
+  CHPP_Start
+| CHPP_input
+| CHPP_input1 (n : nat)
+| CHPP_input2 (n : nat)
+| CHPP_output
+| CHPP_output1 (n : nat)
+| CHPP_output2 (n : nat).
+
+Global Instance chat_server_petri_places_eqdec :
+  EqDecision chat_server_petri_places.
+Proof. solve_decision. Qed.
+
+Instance chat_server_petri_placesC : PlacesC :=
+  {| Places := chat_server_petri_places |}.
+
+Inductive chat_server_petri_base mixer μ1 μ2 : PetriNet :=
+| chat_server_petri_start_split :
+    chat_server_petri_base mixer μ1 μ2 (SplitTr CHPP_Start CHPP_input CHPP_output)
+| chat_server_petri_input_split :
+    chat_server_petri_base mixer μ1 μ2
+                      (SplitTr CHPP_input (CHPP_input1 0) (CHPP_input2 0))
+| chat_server_petri_output_split :
+    chat_server_petri_base mixer μ1 μ2
+                      (SplitTr CHPP_output (CHPP_output1 0) (CHPP_output2 0))
+| chat_server_petri_input1 n :
+    chat_server_petri_base mixer μ1 μ2
+                      (IOTr (CHPP_input1 n) read_nick1 UnitV (Snth n μ1)
+                            (CHPP_input1 (S n)))
+| chat_server_petri_input2 n :
+    chat_server_petri_base mixer μ1 μ2
+                      (IOTr (CHPP_input2 n) read_nick2 UnitV (Snth n μ2)
+                            (CHPP_input2 (S n)))
+| chat_server_petri_output1 n :
+    chat_server_petri_base mixer μ1 μ2
+                      (IOTr (CHPP_output1 n) write_nick1
+                            (Snth n (Smix mixer μ1 μ2))
+                            UnitV
+                            (CHPP_output1 (S n)))
+| chat_server_petri_output2 n :
+    chat_server_petri_base mixer μ1 μ2
+                      (IOTr (CHPP_output2 n) write_nick2
+                            (Snth n (Smix mixer μ1 μ2))
+                            UnitV
+                            (CHPP_output2 (S n))).
+
+Definition chat_server_petri μ1 μ2 : PetriNet :=
+  λ T, ∃ mixer, chat_server_petri_base mixer μ1 μ2 T.
+
+(* Lemma chat_server_petri_det_io mixer μ1 μ2 : *)
+(*   (∀ p t v v' q, *)
+(*       chat_server_petri mixer μ1 μ2 (IOTr p t v v' q) → *)
+(*       (∀ t1 v1 v1' q1, chat_server_petri mixer μ1 μ2 (IOTr p t1 v1 v1' q1) → *)
+(*                        t1 = t ∧ v1 = v ∧ v1' = v' ∧ q1 = q) ∧ *)
+(*       (∀ q1 q2, chat_server_petri mixer μ1 μ2 (SplitTr p q1 q2) → False) ∧ *)
+(*       (∀ p2 q, chat_server_petri mixer μ1 μ2 (JoinTr p p2 q) → False)). *)
+(* Proof. *)
+(*   intros ? ? ? ? ? Hp; inversion Hp; clear Hp; subst; (split; [|split]); *)
+(*     intros; *)
+(*     match goal with *)
+(*     | H : chat_server_petri _ _ _ _ |- _ => inversion H; subst; auto *)
+(*     end. *)
+(* Qed. *)
+
+(* Lemma chat_server_petri_det_split mixer μ1 μ2 : *)
+(*   (∀ p q1 q2, *)
+(*       chat_server_petri mixer μ1 μ2 (SplitTr p q1 q2) → *)
+(*       (∀ t1 v1 v1' q1, chat_server_petri mixer μ1 μ2 (IOTr p t1 v1 v1' q1) → False) *)
+(*       ∧ (∀ q1' q2', chat_server_petri mixer μ1 μ2 (SplitTr p q1' q2') → *)
+(*                     q1' = q1 ∧ q2' = q2) ∧ *)
+(*       (∀ p2 q, chat_server_petri mixer μ1 μ2 (JoinTr p p2 q) → False)). *)
+(* Proof. *)
+(*   intros ? ? ? Hp; inversion Hp; clear Hp; subst; (split; [|split]); *)
+(*     intros; *)
+(*     match goal with *)
+(*     | H : chat_server_petri _ _ _ _ |- _ => inversion H; subst; auto *)
+(*     end. *)
+(* Qed. *)
+
+(* Definition chat_server_petri_start_val := *)
+(*   λ p, match p with CHPP_Start => 1 | _ => 0 end. *)
+
+(* correct the statement, p must be reachable from start! *)
+Lemma chat_server_petri_ResultDet μ1 μ2 p :
+  ResultDet (Traces (chat_server_petri μ1 μ2) p).
+Proof.
+  (* intros t v v' v'' τ τ' τ'' Hτ. *)
+  (* remember (τ ++ (t, v, v') :: τ') as io. *)
+  (* revert τ t v v' v'' τ' Heqio. *)
+  (* induction Hτ as [| ? ? ? ? ? ? ? Hτio | | |] => τ1 t1 v1 v1' v1'' τ1' Heqio Hτ''. *)
+  (* - by destruct τ1. *)
+  (* - inversion Hτ''. *)
+  (*   + by destruct τ1. *)
+  (*   + destruct τ1 as [|[[? ?] ?] τ1]; simpl in *; inversion Heqio; simplify_eq. *)
+  (*     * admit. *)
+  (*     *  *)
+Admitted.
+
+Lemma Recive_from_nick (b : bool) `{inG Σ (authUR (ofe_funUR (λ _ : Places, natUR)))}
+      γ μ1 μ2 :
+  let _ := {| γPN := γ; ThePetriNet := chat_server_petri μ1 μ2 |}in
+  (ReceiveFromNick (if b then (CHPP_input1 0) else (CHPP_input2 0))
+                   (BoolV b) (if b then μ1 else μ2))%I.
+Proof.
+  pose ({| γPN := γ; PNI_exclG := H;
+           ThePetriNet := chat_server_petri μ1 μ2 |}).
+  set (Φ := (λ pμ : @place_stream chat_server_petri_placesC,
+                      ∃ n, ⌜pμ.1 = (if b then CHPP_input1 n else CHPP_input2 n)
+                           ∧ pμ.2 = Sdrop n (if b then μ1 else μ2)⌝)%I
+            : place_stream → iProp Σ).
+  assert (NonExpansive Φ).
+  { by intros n [? ?] [? ?] [?%leibniz_equiv ?%leibniz_equiv];
+      simpl in *; subst. }
+  iApply (greatest_fixpoint_coind _ Φ); simpl; eauto.
+  iAlways. iIntros ([? ?]); iDestruct 1 as %[n [Hn Hμ]]; simpl in *; subst.
+  rewrite /IO_pre_sequence.
+  iExists (if b then CHPP_input1 (S n) else CHPP_input2 (S n)); iSplit; simpl.
+  + iPureIntro. rewrite Snth_Sdrop; destruct b; exists (Sconst true); constructor.
+  + iExists (S n); iPureIntro; split; simpl; auto.
+Qed.
+
+Lemma Send_to_nick (b : bool) `{inG Σ (authUR (ofe_funUR (λ _ : Places, natUR)))}
+      γ μ1 μ2 μ :
+  interleaving μ1 μ2 μ →
+  let _ := {| γPN := γ; ThePetriNet := chat_server_petri μ1 μ2 |}in
+  (SendToNick (if b then (CHPP_output1 0) else (CHPP_output2 0)) (BoolV b) μ)%I.
+Proof.
+  pose ({| γPN := γ; PNI_exclG := H;
+           ThePetriNet := chat_server_petri μ1 μ2 |}).
+  set (Φ := (λ pμ : @place_stream chat_server_petri_placesC,
+                      ∃ n, ⌜pμ.1 = (if b then CHPP_output1 n else CHPP_output2 n)
+                           ∧ pμ.2 = Sdrop n μ⌝)%I
+            : place_stream → iProp Σ).
+  assert (NonExpansive Φ).
+  { by intros n [? ?] [? ?] [?%leibniz_equiv ?%leibniz_equiv];
+      simpl in *; subst. }
+  intros Hinr; simpl.
+  iApply (greatest_fixpoint_coind _ Φ); simpl; eauto.
+  iAlways. iIntros ([? ?]); iDestruct 1 as %[n [Hn Hμ]]; simpl in *; subst.
+  rewrite /IO_pre_sequence.
+  iExists (if b then CHPP_output1 (S n) else CHPP_output2 (S n)); iSplit; simpl.
+  + iPureIntro. rewrite Snth_Sdrop. destruct Hinr as [mixer <-].
+    destruct b; exists mixer; econstructor.
+  + iExists (S n); iPureIntro; split; simpl; auto.
+Qed.
+
+Theorem wp_closed_concrete_serverChatRoom
+        `{heapIPreIOG Σ}
+        `{channelIG Σ}
+        `{inG Σ (authUR (ofe_funUR (λ p : Places, natUR)))}
+        μ1 μ2 :
+  (|={⊤}=> ∃ γio, let _ := make_heapIG γio in
+                 |={⊤}=> ∃ _ : petrinetIG Σ,
+     FullIO (Traces (chat_server_petri μ1 μ2)
+                    (singVAL CHPP_Start))
+            ∗ WP concrete_serveChatRoom {{ _, False }})%I.
+Proof.
+  iIntros "".
+  pose (Traces (chat_server_petri μ1 μ2)
+                (singVAL CHPP_Start)) as ios.
+  iMod (@own_alloc _ io_monoid _
+                   (● Excl' (ios : leibnizC ioSpec) ⋅
+                      ◯ Excl' (ios : leibnizC ioSpec))) as (γio) "[HFI HOI]";
+    first done.
+  iModIntro. iExists _. pose (make_heapIG γio). iFrame.
+  iMod (PetriNetInv_alloc with "HOI") as (γpn) "[#HPi HOV]".
+  { apply chat_server_petri_ResultDet. }
+  pose ({| PNI_exclG := _; γPN := γpn; ThePetriNet := chat_server_petri μ1 μ2|})
+    as PN.
+  iModIntro. iExists PN.
+  iAssert (@Token chat_server_petri_placesC _ _ _ CHPP_Start) with "[$HOV]"
+    as "HOS"; first done.
+  iMod (petrinet_split with "[HOS]") as "[HI HO]"; [| by iFrame |].
+  { exists (Sconst true); apply chat_server_petri_start_split. }
+  iMod (petrinet_split with "[HI]") as "[HI1 HI2]"; [| by iFrame |].
+  { exists (Sconst true); apply chat_server_petri_input_split. }
+  iPoseProof (Recive_from_nick true γpn μ1 μ2) as "HRFN1".
+  iPoseProof (Recive_from_nick false γpn μ1 μ2) as "HRFN2".
+  iApply (@wp_concrete_serverChatRoom
+            _ _ chat_server_petri_placesC _ _
+            (CHPP_input1 0) (CHPP_input2 0) CHPP_output μ1 μ2 with "[-]");
+    last done.
+  iFrame; iFrame "#".
+  iIntros (μ Hintr).
+  iExists _, _; simpl.
+  iSplit.
+  { iPureIntro. eexists (Sconst true); econstructor. }
+  iSplitL.
+  by iApply (Send_to_nick true).
+  by iApply (Send_to_nick false).
+Qed.
+
+Theorem concrete_serverChatRoom_safe :
+        fully_erased_safe
+          concrete_serveChatRoom
+          (λ T, ∃ μ1 μ2, (@Traces
+                            chat_server_petri_placesC
+                            (chat_server_petri μ1 μ2) (singVAL CHPP_Start)) T).
+Proof.
+  eapply fully_erased_safe_equiv;
+    last apply (fully_erased_safe_union concrete_serveChatRoom
+         (λ M, ∃ μ1 μ2 : Stream val, M ≡
+                        Traces (chat_server_petri μ1 μ2)
+                                (@singVAL chat_server_petri_placesC
+                                          CHPP_Start))).
+  - intros T; split.
+    + intros (μ1 & μ2 & ?).
+      exists (λ T, Traces (chat_server_petri μ1 μ2)
+                   (@singVAL chat_server_petri_placesC CHPP_Start) T).
+      split; eauto.
+    + intros [M [(μ1 & μ2 & HMeq) HM]]. eexists _, _; by apply HMeq.
+  - intros M (μ1 & μ2 & HM).
+    apply leibniz_equiv in HM; subst.
+    pose (#[IoΣ; petrinetΣ; channelΣ]) as Σ.
+    apply (adequacy Σ _ ((λ _, False))%I).
+    { admit. }
+    intros Hig.
+    iIntros "".
+    iMod (wp_closed_concrete_serverChatRoom μ1 μ2) as (γio) "Hlm".
+    iMod ("Hlm") as (HIG) "[HFIO HWP]".
+    iModIntro; iExists _; iFrame.
+Admitted.
